some progress on proving subst factors through compilation

Hs/Metatheory/SubstitutionCompile.lean
@@ -5,43 +5,326 @@ import Hs.Metatheory.TypeMatch
 import Hs.Metatheory.Weaken
 import Hs.Metatheory.WeakenCompile
 import Hs.Metatheory.Substitution
+-- import Hs.Metatheory.Soundness1
 import Hs.Algorithm
 
+set_option maxHeartbeats 1000000
 
 def subst_compile_kind : {Γ Δ : Ctx HsTerm} -> {σ : Subst HsTerm} -> {σ' : Subst Term} ->
-  (∀ n y, σ n = .re y -> (Γ d@ n).apply σ = Δ d@ y) ->
-  (∀ n t T, σ n = .su t -> .some T = (Γ d@ n).get_type -> Δ ⊢κ t : ([σ]T)) ->
-  (∀ n, Γ.is_stable n -> ∃ y, σ n = .re y) ->
-
   (j : Γ ⊢κ t : k) ->
   compile_kind Γ t k j = .some t' ->
   ⊢s Δ ->
 
   (sj : Δ ⊢κ ([σ]t) : ([σ]k)) ->
   compile_kind Δ ([σ]t) ([σ]k) sj = .some ([σ']t') := by
+intro Γ Δ σ σ' j cj wf sj
+induction Γ, t, k, j using compile_kind.induct generalizing Δ t'
+case _ Γ j =>
+  unfold compile_kind; cases sj; simp;
+  unfold compile_kind at cj; cases cj; simp;
+case _ Γ A B j1 j2 ih1 ih2 =>
+  unfold compile_kind at cj; simp at cj;
+  rw[Option.bind_eq_some] at cj;
+  cases cj; case _ A' cj =>
+  cases cj; case _ cA cj =>
+  rw[Option.bind_eq_some] at cj;
+  cases cj; case _ B' cj =>
+  cases cj; case _ cB cj =>
+  cases cj
+  cases sj; case _ jA' jB' =>
+  unfold compile_kind; simp;
+  rw[Option.bind_eq_some];
+  exists ([σ']A');
+  constructor;
+  apply @ih1 A' Δ cA wf jA'
+  rw[Option.bind_eq_some];
+  exists ([σ']B')
+  constructor;
+  apply @ih2 B' Δ cB wf jB'
+  simp
 
-sorry
 
+def subst_compile_type : {Γ Δ : Ctx HsTerm} -> {σ : Subst HsTerm} -> {σ' : Subst Term} ->
+  (∀ (Γ : Ctx HsTerm) (h1 h2 : ⊢s Γ), h1 = h2) ->
+  (f1 : ∀ n y, σ n = .re y -> (Γ d@ n).apply σ = Δ d@ y) ->
 
+  (f2 : ∀ n t T, σ n = .su t -> .some T = (Γ d@ n).get_type -> Δ ⊢τ t : ([σ]T)) ->
 
+  (f3 : ∀ n, Γ.is_stable n -> ∃ y, σ n = .re y) ->
+
+  -- Substitutions are related via compilation
+  -- (∀ n y, σ n = .re y -> σ' n = .re y) ->
+  -- (∀ n t, σ n = .su t -> ∃ t', σ' n = .su t') ->
+  -- (∀ i t wt t' wt',
+  --    σ' i = .su t' ->
+  --    σ i = .su t ->
+  --    (j : Γ ⊢τ t : k) ->
+  --    (j' : Δ ⊢τ ([σ]t) : ([σ]k)) ->
+  --    compile_type Γ t k j = .some wt ->
+  --    compile_type Δ ([σ]t) ([σ]k) j' = .some wt' ->
+  --    [σ']wt = wt'
+  -- ) ->
+
+  (j : Γ ⊢τ t : k) ->
+  compile_type Γ t k j = .some t' ->
+  (wf : ⊢s Δ) ->
+
+  (sj : Δ ⊢τ ([σ]t) :  ([σ] k)) ->
+
+  compile_type Δ ([σ]t) ([σ]k) sj = .some ([σ']t')
+:= by
+intro Γ Δ σ σ' h f1 f2 f3 /- f4 f5 f6 -/ j cj wf sj -- e
+induction Γ, t, k, j using compile_type.induct generalizing Δ t' σ σ'
+case _ Γ T n wf' test gt ck  =>
+  have j := HsJudgment.varTy wf' test gt ck
+  unfold compile_type at cj; simp at cj;
+  rw[Option.bind_eq_some] at cj;
+  cases cj; case _ T' cj =>
+  cases cj; case _ cT cj =>
+  cases cj
+  generalize zdef : σ n = y at *;
+  cases y;
+  case _ x =>
+    -- have lem1 := f4 n x zdef;
+    -- simp; rw[lem1]; simp;
+    -- have sj' := sj
+    -- simp at sj'; rw[zdef] at sj'; simp at sj'
+    -- have lem2 := f2 n
+    sorry
+  case _ st =>
+    -- have lemf5 := f5 n st zdef
+    -- cases lemf5; case _ st' lemf5 =>
+    -- have lemf6 := f6 n st
+    sorry
+case _ Γ B f A a jf ja jA jB ih1 ih2 => -- appk
+  generalize ej : hs_subst_type f1 f2 f3 (jf.appk ja jA jB) wf = sj' at *;
+  have u := types_have_unique_judgments h sj sj'; cases u;
+  unfold compile_type at cj; simp at cj;
+  rw[Option.bind_eq_some] at cj;
+  cases cj; case _ A' cj =>
+  cases cj; case _ cA cj =>
+  rw[Option.bind_eq_some] at cj;
+  cases cj; case _ B' cj =>
+  cases cj; case _ cB cj =>
+  rw[Option.bind_eq_some] at cj;
+  cases cj; case _ f' cj =>
+  cases cj; case _ cf cj =>
+  rw[Option.bind_eq_some] at cj;
+  cases cj; case _ a' cj =>
+  cases cj; case _ ca cj =>
+  cases cj;
+  rw[<-ej]
+  unfold compile_type; simp; unfold hs_subst_type; simp;
+  rw[Option.bind_eq_some]
+  exists([σ']A')
+  constructor;
+  apply subst_compile_kind jA cA wf
+  rw[Option.bind_eq_some]
+  exists([σ']B')
+  constructor;
+  apply subst_compile_kind jB cB wf
+  rw[Option.bind_eq_some]
+  exists([σ']f')
+  constructor;
+  apply @ih1 f' Δ σ σ' f1 f2 f3 cf wf
+  rw[Option.bind_eq_some]
+  exists ([σ']a')
+  constructor
+  simp
+  apply @ih2 a' Δ σ σ' f1 f2 f3 ca wf
+  simp
+
+case _ Γ A B jA jB ih => -- allt
+  have lem : (Option.map (λ x => [σ'] x) (compile_type Γ (`∀{A} B) `★ (jA.allt jB)))
+             = (Option.map (λ x => [σ'] x) (.some t')) := by rw [cj]
+  have lem' : (Option.map (λ x => [σ'] x) (.some t')) = .some ([σ'] t') := by  simp
+  rw[lem'] at lem; rw[<-lem];
+  simp
+  have lem'' := compile_preserves_type_shape_all (jA.allt jB) cj;
+  cases lem''; case _ A' lem'' =>
+  cases lem''; case _ B' lem'' =>
+  cases lem''
+  -- cases e;
+  rw[cj]; simp;
+  unfold compile_type at cj; simp at cj;
+  rw[Option.bind_eq_some] at cj;
+  cases cj; case _ A' cj =>
+  cases cj; case _ cA cj =>
+  rw[Option.bind_eq_some] at cj;
+  cases cj; case _ B' cj =>
+  cases cj; case _ cB cj =>
+  cases cj;
+  generalize ej : hs_subst_type f1 f2 f3 (jA.allt jB) wf = sj' at *;
+  have u := types_have_unique_judgments h sj sj'; cases u;
+  unfold compile_type; simp; unfold hs_subst_type at ej; simp at ej; rw[<-ej]
+  rw[Option.bind_eq_some]
+  exists ([σ']A')
+  constructor;
+  apply subst_compile_kind jA cA wf
+
+  rw[Option.bind_eq_some]
+  exists ([^σ'] B')
+  constructor;
+
+  have lem := hs_subst_kind f1 f3 jA wf; rw[HsTerm.subst_HsKind] at lem;
+  have wf'' : ⊢s (.kind ([σ]A) :: Δ) := by apply HsJudgment.wfkind; assumption; assumption
+  generalize wfh : (hs_subst_kind f1 f3 jA wf).wfkind wf = wf' at *;
+  generalize f1e : hs_lift_subst_rename (.kind A) f1 = f1' at *
+  generalize f2e : hs_lift_subst_replace (.kind A) wf'' f2 = f2' at *
+  generalize f3e : hs_lift_subst_stable (.kind A) f3 = f3' at *
+
+  apply  @ih B' (.kind ([σ]A) :: Δ) (^σ) (^σ') f1' f2' f3' cB wf'
+  simp;
+case _ Γ A B jA jB ih1 ih2 => -- arrow
+  have lem : (Option.map (λ x => [σ'] x) (compile_type Γ (A → B) `★ (jA.arrow jB)))
+             = (Option.map (λ x => [σ'] x) (.some t')) := by rw [cj]
+  have lem' : (Option.map (λ x => [σ'] x) (.some t')) = .some ([σ'] t') := by  simp
+  rw[lem'] at lem; rw[<-lem];
+  simp
+  have lem'' := compile_preserves_type_shape_arrow (jA.arrow jB) cj;
+  cases lem''; case _ A' lem'' =>
+  cases lem''; case _ B' lem'' =>
+  cases lem''; case _ jA' lem'' =>
+  cases lem''; case _ jB' lem'' =>
+  cases lem''; case _ e lem'' =>
+  cases e
+  cases lem''; case _ cjA cjB =>
+  have u := types_have_unique_judgments h jA jA'; cases u
+  have u := types_have_unique_judgments h jB jB'; cases u
+  rw[cj]; simp;
+  generalize ej : hs_subst_type f1 f2 f3 (jA.arrow jB) wf = sj' at *;
+  have u := types_have_unique_judgments h sj sj'; cases u;
+
+  unfold compile_type; simp; rw [<-ej]; unfold hs_subst_type; simp;
+  rw[Option.bind_eq_some]
+  exists ([σ']A')
+  constructor;
+  cases sj; case _ sjA sjB =>
+    clear ih2;
+    unfold hs_subst_type at ej; simp at ej; cases ej;
+    apply @ih1 A' Δ σ σ' f1 f2 f3 /- f4 f5 f6-/ cjA wf
+
+  rw[Option.bind_eq_some]
+  exists ([^σ'] B')
+  constructor;
+  clear ih1;
+  unfold hs_subst_type at ej; simp at ej; cases ej;
+  have wf' : ⊢s (.empty :: Δ) := by constructor; assumption
+  have f1' := hs_lift_subst_rename .empty f1
+
+  generalize fh : @hs_lift_subst_replace σ Δ Γ .type .empty wf' f2 = f2' at *;
+  have ef2 : @hs_lift_subst_replace σ Δ Γ .type .empty wf' f2 = f2' := by
+    rw [fh]
+
+  have f3' := hs_lift_subst_stable .empty f3
+
+  apply  @ih2 B' (.empty :: Δ) (^σ) (^σ') f1' f2' f3' cjB wf'
+  simp
+
+case _ Γ A B jA vhv jB ih1 ih2 =>  -- farrow
+  have lem : (Option.map (λ x => [σ'] x) (compile_type Γ (A ⇒ B) `★ (.farrow jA vhv jB)))
+             = (Option.map (λ x => [σ'] x) (.some t')) := by rw [cj]
+  have lem' : (Option.map (λ x => [σ'] x) (.some t')) = .some ([σ'] t') := by  simp
+  rw[lem'] at lem; rw[<-lem];
+  simp
+  have lem'' := compile_preserves_type_shape_arrow (jA.arrow jB) cj;
+  cases lem''; case _ A' lem'' =>
+  cases lem''; case _ B' lem'' =>
+  cases lem''; case _ jA' lem'' =>
+  cases lem''; case _ jB' lem'' =>
+  cases lem''; case _ e lem'' =>
+  cases e
+  cases lem''; case _ cjA cjB =>
+  have u := types_have_unique_judgments h jA jA'; cases u
+  have u := types_have_unique_judgments h jB jB'; cases u
+  rw[cj]; simp;
+  generalize ej : hs_subst_type f1 f2 f3 (jA.farrow vhv jB) wf = sj' at *;
+  have u := types_have_unique_judgments h sj sj'; cases u;
+
+  unfold compile_type; simp; rw [<-ej]; unfold hs_subst_type; simp;
+  rw[Option.bind_eq_some]
+  exists ([σ']A')
+  constructor;
+  cases sj; case _ sjA sjB =>
+    clear ih2;
+    unfold hs_subst_type at ej; simp at ej; cases ej;
+    apply @ih1 A' Δ σ σ' f1 f2 f3 /- f4 f5 f6-/ cjA wf
+
+  rw[Option.bind_eq_some]
+  exists ([^σ'] B')
+  constructor;
+  clear ih1;
+  unfold hs_subst_type at ej; simp at ej; cases ej;
+  have wf' : ⊢s (.empty :: Δ) := by constructor; assumption
+  have f1' := hs_lift_subst_rename .empty f1
+
+  generalize fh : @hs_lift_subst_replace σ Δ Γ .type .empty wf' f2 = f2' at *;
+  have ef2 : @hs_lift_subst_replace σ Δ Γ .type .empty wf' f2 = f2' := by
+    rw [fh]
+
+  have f3' := hs_lift_subst_stable .empty f3
+
+  apply  @ih2 B' (.empty :: Δ) (^σ) (^σ') f1' f2' f3' cjB wf'
+  simp
 
 
 theorem compile_beta_kind_type :
+  (∀ (Γ : Ctx HsTerm) (h1 h2 : ⊢s Γ), h1 = h2) ->
   (j1 : (.kind A::Γ) ⊢τ b : B) ->
   compile_type (.kind A::Γ) b B j1 = .some b' ->
   (j2 : Γ ⊢τ t : A) ->
   compile_type Γ t A j2 = .some t' ->
   (j3 : Γ ⊢τ (b β[t]) : (B β[t])) ->
-  compile_type Γ (b β[t]) (B β[t]) j3 = .some (b' β[t']) := by sorry
-
+  compile_type Γ (b β[t]) (B β[t]) j3 = .some (b' β[t']) := by
+intro h j1 cj1 j2 cj2 j3;
+apply @subst_compile_type b B b' (.kind A :: Γ) Γ (.su t :: I) (.su t' :: I) h
+case _ =>
+  intro n y h1;
+  cases n <;> simp at *; subst h1
+  case _ n =>
+    rw [Frame.apply_compose]; simp
+case _ =>
+  intro n s T h1 h2
+  cases n <;> simp at *; subst h1
+  injection h2 with e; subst e; simp
+  apply j2
+case _ =>
+  intro n h1
+  cases n <;> simp at *
+  rw [Frame.is_stable_stable] at h1
+  unfold Frame.is_stable at h1
+  simp at h1
+assumption
+apply hs_judgment_ctx_wf .type j2
 
 theorem compile_beta_empty_type :
+  (∀ (Γ : Ctx HsTerm) (h1 h2 : ⊢s Γ), h1 = h2) ->
   (j1 : (.empty::Γ) ⊢τ b : B) ->
   compile_type (.empty::Γ) b B j1 = .some b' ->
   (j2 : Γ ⊢τ t : A) ->
   compile_type Γ t A j2 = .some t' ->
   (j3 : Γ ⊢τ (b β[t]) : (B β[t])) ->
-  compile_type Γ (b β[t]) (B β[t]) j3 = .some (b' β[t']) := by sorry
+  compile_type Γ (b β[t]) (B β[t]) j3 = .some (b' β[t']) := by
+intro h j1 cj1 j2 cj2 j3;
+apply @subst_compile_type b B b' (.empty :: Γ) Γ (.su t :: I) (.su t' :: I) h
+case _ =>
+  intro n y h1;
+  cases n <;> simp at *; subst h1
+  case _ n =>
+    rw [Frame.apply_compose]; simp
+case _ =>
+  intro n s T h1 h2
+  cases n <;> simp at *; subst h1
+  unfold Frame.get_type at h2; simp at h2
+case _ =>
+  intro n h1
+  cases n <;> simp at *
+  rw [Frame.is_stable_stable] at h1
+  unfold Frame.is_stable at h1
+  simp at h1
+assumption
+apply hs_judgment_ctx_wf .type j2
+
 
 theorem compile_beta_empty_term :
   (j1 : (.empty::Γ) ⊢τ b : B) ->
